lots of cleanup

src/TL.lean
@@ -1,11 +1,17 @@
+/-
+Definitions of a type theory
+
+Author: Billy Price
+-/
+
 import data.finset
 namespace TT
 
 inductive type : Type
-| One | Omega | Prod (A B : type)| Pow (A : type)
+| Unit | Omega | Prod (A B : type)| Pow (A : type)
 
 notation `Ω` := type.Omega
-notation `𝟙` := type.One
+def Unit := type.Unit
 infix `××`:max := type.Prod
 prefix 𝒫 :max := type.Pow
 
@@ -18,223 +24,197 @@ inductive term : Type
 | and  : term → term → term
 | or   : term → term → term
 | imp  : term → term → term
+| elem : term → term → term
+| pair : term → term → term
 | var  : ℕ → term
 | comp : term → term
 | all  : term → term
 | ex   : term → term
-| elem : term → term → term
-| prod : term → term → term
-
-open term
 
 -- * * * * * * * * * * * * * * * * * * * * * * * * * * * * * * * * * * * * * * * 
 -- Notation and derived operators 
 -- * * * * * * * * * * * * * * * * * * * * * * * * * * * * * * * * * * * * * * * 
 
-notation `<0>` := var 0
-notation `<1>` := var 1
-notation `<2>` := var 2
-notation `<3>` := var 3
-notation `<4>` := var 4
-notation `<5>` := var 5
-notation `<6>` := var 6
-notation `<7>` := var 7
-notation `<8>` := var 8
-notation `<9>` := var 9
+notation `𝟘` := term.var 0
+notation `𝟙` := term.var 1
+notation `𝟚` := term.var 2
+notation `𝟛` := term.var 3
+notation `𝟜` := term.var 4
+notation `𝟝` := term.var 5
 
-notation `⁎` := star    -- input \asterisk
-notation `⊤` := top     --       \top
-notation `⊥` := bot     -- input \bot
-infixr ` ⟹ `:60 := imp -- input \==>
-infixr ` ⋀ ` :70 := and -- input \glb or \sqcap
-infixr ` ⋁ ` :59 := or  -- input \lub or ⋁
+notation `⁎` := term.star    -- input \asterisk
+notation `⊤` := term.top     --       \top
+notation `⊥` := term.bot     -- input \bot
+infixr ` ⟹ `:60 := term.imp -- input \==>
+infixr ` ⋀ ` :70 := term.and -- input \And or \bigwedge
+infixr ` ⋁ ` :59 := term.or  -- input \Or or \bigvee
 
 def not (p : term) := p ⟹ ⊥
-prefix `∼`:max := not -- input \~, the ASCII character ~ has too low precedence
+prefix `∼`:max := not -- input \~
 
-def biimp (p q: term) := (p ⟹ q) ⋀ (q ⟹ p)
-infix ` ⇔ `:60 := biimp -- input \<=>
+def iff (p q: term) := (p ⟹ q) ⋀ (q ⟹ p)
+infix ` ⇔ `:60 := iff -- input \<=>
 
-infix ∈ := elem
-infix ∉ := λ a, λ α, not (elem a α)
-notation `⟦` φ `⟧` := comp φ
+infix ∈ := term.elem
+infix ∉ := λ a α, not (term.elem a α)
+notation `⟦` φ `⟧` := term.comp φ
 
-infix `××` :max := prod
+notation `⟪` a `,` b `⟫` := term.pair a b 
 
-prefix `∀'`:1 := all 
-prefix `∃'`:2 := ex
+prefix `∀'`:1 := term.all 
+prefix `∃'`:2 := term.ex
 
-def eq (a : term) (a' : term) : term := ∀' (a ∈ <0>) ⇔ (a' ∈ <0>)
+def eq (a₁ a₂ : term) : term := ∀' (a₁ ∈ 𝟘) ⇔ (a₂ ∈ 𝟘)
 infix `≃` :50 := eq
 
-def singleton (a : term) := ⟦a ≃ (<0>)⟧
+def singleton (a : term) := ⟦a ≃ (𝟘)⟧
 
 def ex_unique (φ : term) : term :=
-  ∃' ⟦φ⟧ ≃ singleton (<3>)
+  ∃' ⟦φ⟧ ≃ singleton (𝟛)
 prefix `∃!'`:2 := ex_unique
 
 def subseteq (α : term) (β : term) : term :=
-  ∀' (<0> ∈ α) ⟹ (<0> ∈ β)
+  ∀' (𝟘 ∈ α) ⟹ (𝟘 ∈ β)
 infix ⊆ := subseteq
 
+def set_prod {A B : type} (α β : term) : term :=
+  ⟦∃' ∃' (𝟙 ∈ α) ⋀ (𝟘 ∈ β) ⋀ (𝟛 ≃ ⟪𝟚,𝟙⟫)⟧
+
 -- * * * * * * * * * * * * * * * * * * * * * * * * * * * * * * * * * * * * * * *
+open term
 
-inductive WF : context → term → type → Prop
-| star {Γ}           : WF Γ term.star 𝟙
-| top  {Γ}           : WF Γ term.top Ω
-| bot  {Γ}           : WF Γ term.bot Ω
-| and  {Γ e₁ e₂}     : WF Γ e₁ Ω → WF Γ e₁ Ω → WF Γ (e₁ ⋀ e₂) Ω
-| or   {Γ e₁ e₂}     : WF Γ e₁ Ω → WF Γ e₁ Ω → WF Γ (e₁ ⋁ e₂) Ω
-| imp  {Γ e₁ e₂}     : WF Γ e₁ Ω → WF Γ e₁ Ω → WF Γ (e₁ ⟹ e₂) Ω
-| var  {Γ n A}       : list.nth Γ n = some A → WF Γ (var n) A
-| comp {Γ e A}       : WF (A::Γ) e Ω → WF Γ ⟦e⟧ (𝒫 A)
-| all  {Γ e A}       : WF (A::Γ) e Ω → WF Γ (∀' e) Ω
-| ex   {Γ e A}       : WF (A::Γ) e Ω → WF Γ (∃' e) Ω
-| elem {Γ e₁ e₂ A}   : WF Γ e₁ A → WF Γ e₂ (𝒫 A) → WF Γ (e₁ ∈ e₂) Ω
-| prod {Γ e₁ e₂ A B} : WF Γ e₁ A → WF Γ e₂ B → WF Γ (prod e₁ e₂) (A ×× B)
 
-lemma WF_and_left {Γ p q} : WF Γ (p ⋀ q) Ω → WF Γ p Ω := sorry
-lemma WF_and_right {Γ p q} : WF Γ (p ⋀ q) Ω → WF Γ q Ω := sorry
-lemma WF_or_left {Γ p q} : WF Γ (p ⋁ q) Ω → WF Γ p Ω := sorry
-lemma WF_or_right {Γ p q} : WF Γ (p ⋁ q) Ω → WF Γ q Ω := sorry
-lemma WF_imp_left {Γ p q} : WF Γ (p ⟹ q) Ω → WF Γ p Ω := sorry
-lemma WF_imp_right {Γ p q} : WF Γ (p ⟹ q) Ω → WF Γ q Ω := sorry
+section wellformedness
 
-#check @WF.and
+  inductive WF : context → type → term → Prop
+  | star {Γ}         : WF Γ Unit ⁎
+  | top  {Γ}         : WF Γ Ω ⊤
+  | bot  {Γ}         : WF Γ Ω ⊥
+  | and  {Γ p q}     : WF Γ Ω p → WF Γ Ω q → WF Γ Ω (p ⋀ q)
+  | or   {Γ p q}     : WF Γ Ω p → WF Γ Ω q → WF Γ Ω (p ⋁ q)
+  | imp  {Γ p q}     : WF Γ Ω p → WF Γ Ω q → WF Γ Ω (p ⟹ q)
+  | elem {Γ A a α}   : WF Γ A a → WF Γ (𝒫 A) α → WF Γ Ω (a ∈ α)
+  | pair {Γ A B a b} : WF Γ A a → WF Γ B b → WF Γ (A ×× B) ⟪a,b⟫
+  | var  {Γ A n}     : list.nth Γ n = some A → WF Γ A (var n)
+  | comp {Γ A φ}     : WF (A::Γ) Ω φ → WF Γ (𝒫 A) ⟦φ⟧
+  | all  {Γ A φ}     : WF (A::Γ) Ω φ → WF Γ Ω (∀' φ)
+  | ex   {Γ A φ}     : WF (A::Γ) Ω φ → WF Γ Ω (∃' φ)
 
-def lift (d : ℕ): ℕ → term → term
-| k star       := star
-| k top        := top
-| k bot        := bot
-| k (p ⋀ q)    := (lift k p) ⋀ (lift k q)
-| k (p ⋁ q)    := (lift k p) ⋁ (lift k q)
-| k (p ⟹ q)    := (lift k p) ⟹ (lift k q)
-| k (var m)    := if m≥k then var (m+d) else var m
-| k ⟦φ⟧         :=    ⟦lift (k+1) φ⟧
-| k (∀' φ)     := ∀' lift (k+1) φ
-| k (∃' φ)     := ∃' lift (k+1) φ
-| k (a ∈ α)    := (lift k a) ∈ (lift k α)
-| k (prod a b) := prod (lift k a) (lift k b)
 
-def subst_nth : term → ℕ → term → term
-| b n star       := star
-| b n top        := top
-| b n bot        := bot
-| b n (p ⋀ q)    := (subst_nth b n p) ⋀ (subst_nth b n q)
-| b n (p ⋁ q)    := (subst_nth b n p) ⋁ (subst_nth b n q)
-| b n (p ⟹ q)  := (subst_nth b n p) ⟹ (subst_nth b n q)
-| b n (var m)    := if n=m then b else var m
-| b n ⟦φ⟧        :=     ⟦subst_nth (lift 1 0 b) (n+1) φ⟧
-| b n (∀' φ)     := ∀' (subst_nth (lift 1 0 b) (n+1) φ)
-| b n (∃' φ)     := ∃' (subst_nth (lift 1 0 b) (n+1) φ)
-| b n (a ∈ α)    := (subst_nth b n a) ∈ (subst_nth b n α)
-| b n (prod a c) := prod (subst_nth b n a) (subst_nth b n c)
+  variable {Γ : context}
+  variables p q r φ a b α : term
+  variables {A B Ω' : type}
+  -- Ω' is just a fake/variable version of Ω so we don't need to bother proving
+  -- that it must be Ω itself.
 
-def subst (b:term) := subst_nth b 0
+  local notation `ez` := by {intro h, cases h, assumption}
+  lemma WF.and_left   : WF Γ Ω' (p ⋀ q) → WF Γ Ω' p               := ez
+  lemma WF.and_right  : WF Γ Ω' (p ⋀ q) → WF Γ Ω' q               := ez
+  lemma WF.or_left    : WF Γ Ω' (p ⋁ q) → WF Γ Ω' p               := ez
+  lemma WF.or_right   : WF Γ Ω' (p ⋁ q) → WF Γ Ω' q               := ez
+  lemma WF.imp_left   : WF Γ Ω' (p ⟹ q) → WF Γ Ω' p             := ez
+  lemma WF.imp_right  : WF Γ Ω' (p ⟹ q) → WF Γ Ω' q             := ez
+  lemma WF.pair_left  : WF Γ (A ×× B) ⟪a,b⟫ → WF Γ A a            := ez
+  lemma WF.pair_right : WF Γ (A ×× B) ⟪a,b⟫ → WF Γ B b            := ez
+  lemma WF.comp_elim  : WF Γ (𝒫 A) (⟦φ⟧) → WF (A::Γ) Ω φ          := ez
+  lemma WF.all_elim   : WF Γ Ω' (∀' φ) → ∃ A:type, WF (A::Γ) Ω' φ :=
+    by {intro h, cases h, constructor, assumption}
+  lemma WF.ex_elim    : WF Γ Ω' (∀' φ) → ∃ A:type, WF (A::Γ) Ω' φ :=
+    by {intro h, cases h, constructor, assumption}
+  lemma WF.iff_intro : WF Γ Ω p → WF Γ Ω q → WF Γ Ω (p ⇔ q) :=
+    by {intros h₁ h₂, apply WF.and, all_goals {apply WF.imp, assumption, assumption}}
+  lemma WF.iff_elim : WF Γ Ω' (p ⇔ q) → WF Γ Ω' p ∧ WF Γ Ω' q :=
+    by {intro h, apply and.intro, all_goals {cases h, cases h_a, assumption}}
+  lemma WF.eq_intro {Γ} {a₁ a₂} (A : type) : WF ((𝒫 A) :: Γ) A a₁ → WF ((𝒫 A) :: Γ) A a₂ → WF Γ Ω (a₁ ≃ a₂) :=
+    by {intros h₁ h₂, apply WF.all, apply WF.iff_intro, all_goals {apply WF.elem, assumption, apply WF.var, simp}}
 
-def remap_vars : Π k : ℕ, (ℕ → ℕ) → term → term
-| k σ top        := top
-| k σ star       := star
-| k σ bot        := bot
-| k σ (p ⋀ q)   := (remap_vars k σ p) ⋀ (remap_vars k σ q)
-| k σ (p ⋁ q)   := (remap_vars k σ p) ⋁ (remap_vars k σ q)
-| k σ (p ⟹ q)  := (remap_vars k σ p) ⟹ (remap_vars k σ q)
-| k σ (var m)    := var (σ (m+k))
-| k σ ⟦φ⟧         := ⟦remap_vars (k+1) σ φ⟧
-| k σ (∀' φ)     := ∀' remap_vars (k+1) σ φ
-| k σ (∃' φ)     := ∃' remap_vars (k+1) σ φ
-| k σ (a ∈ α)    := (remap_vars k σ a) ∈ (remap_vars k σ α)
-| k σ (prod a b) := prod (remap_vars k σ a) (remap_vars k σ b)
+end wellformedness
 
-inductive proof : context → term → term → Prop
--- c1-3 unecessary?? (because free variables must appear in context)
-| axm        {Γ φ}     : WF Γ φ Ω → proof Γ φ φ
-| vac        {Γ φ}     : WF Γ φ Ω → proof Γ φ term.top
-| abs        {Γ φ}     : WF Γ φ Ω → proof Γ term.bot φ
-| cut        {Γ φ ψ γ} : proof Γ φ ψ → proof Γ ψ γ → proof Γ φ γ
-| and_intro  {Γ p q r} : proof Γ p q → proof Γ p r → proof Γ p (q ⋀ r)  
-| and_left   {Γ p q r} : proof Γ p (q ⋀ r) → proof Γ p q
-| and_right  {Γ p q r} : proof Γ p (q ⋀ r) → proof Γ p r
-| or_intro   {Γ p q r} : proof Γ p r → proof Γ q r → proof Γ (p ⋁ q) r  
-| or_left    {Γ p q r} : proof Γ (p ⋁ q) r → proof Γ p r
-| or_right   {Γ p q r} : proof Γ (p ⋁ q) r → proof Γ q r
-| imp_to_and {Γ p q r} : proof Γ p (q ⟹ r) → proof Γ (p ⋀ q) r
-| and_to_imp {Γ p q r} : proof Γ (p ⋀ q) r → proof Γ p (q ⟹ r)
-| add_var    {Γ φ ψ B} : proof Γ φ ψ → proof (B :: Γ) φ ψ
+section substitution
 
-| apply    {Γ φ ψ b B} :
-    WF Γ b B
-    → proof (B::Γ) φ ψ
-    → proof Γ (subst b φ) (subst b ψ)
+  def lift (d : ℕ) : ℕ → term → term
+  | k ⁎          := ⁎
+  | k ⊤          := ⊤
+  | k ⊥          := ⊥
+  | k (p ⋀ q)    := (lift k p) ⋀ (lift k q)
+  | k (p ⋁ q)    := (lift k p) ⋁ (lift k q)
+  | k (p ⟹ q)   := (lift k p) ⟹ (lift k q)
+  | k (a ∈ α)    := (lift k a) ∈ (lift k α)
+  | k ⟪a,b⟫      := ⟪lift k a, lift k b⟫
+  | k (var m)    := if m≥k then var (m+d) else var m
+  | k ⟦φ⟧         :=    ⟦lift (k+1) φ⟧
+  | k (∀' φ)     := ∀' lift (k+1) φ
+  | k (∃' φ)     := ∃' lift (k+1) φ
 
-| all_elim   {Γ p φ B} : proof Γ p (∀' φ) → proof (B::Γ) p φ
-| all_intro  {Γ p φ B} : proof (B::Γ) p φ → proof Γ p (∀' φ)
-| ex_elim    {Γ p φ B} : proof Γ p (∃' φ) → proof (B::Γ) p φ
-| ex_intro   {Γ p φ B} : proof (B::Γ) p φ → proof Γ p (∃' φ)
+  def subst_nth : ℕ → term → term → term
+  | n x ⁎          := ⁎
+  | n x ⊤          := ⊤
+  | n x ⊥          := ⊥
+  | n x (p ⋀ q)    := (subst_nth n x p) ⋀ (subst_nth n x q)
+  | n x (p ⋁ q)    := (subst_nth n x p) ⋁ (subst_nth n x q)
+  | n x (p ⟹ q)  := (subst_nth n x p) ⟹ (subst_nth n x q)
+  | n x (a ∈ α)    := (subst_nth n x a) ∈ (subst_nth n x α)
+  | n x ⟪a,c⟫      := ⟪subst_nth n x a, subst_nth n x c⟫
+  | n x (var m)    := if n=m then x else var m
+  | n x ⟦φ⟧         :=    ⟦subst_nth (n+1) (lift 1 0 x) φ⟧
+  | n x (∀' φ)     := ∀' (subst_nth (n+1) (lift 1 0 x) φ)
+  | n x (∃' φ)     := ∃' (subst_nth (n+1) (lift 1 0 x) φ)
 
-| comp       {Γ φ A}   :
-    WF (A::A::Γ) φ Ω
-    → proof Γ ⊤
-      (∀' (<0> ∈ ⟦φ⟧) ⇔ (subst <0> φ))
+  def subst := subst_nth 0
 
-| ext                  :
-    proof [] ⊤ $ 
-      ∀' ∀' (∀' (<0> ∈ <2>) ⇔ (<0> ∈ <1>)) ⟹ (<1> ≃ <0>)
+  notation  φ `⁅` b `⁆` := subst b φ
 
-| prop_ext             : proof [] ⊤ ∀' ∀' (<1> ⇔ <0>) ⟹ (<1> ≃ <0>)
-| star_unique          : proof [] ⊤ ∀' (<0> ≃ ⁎)
-| prod_exists_rep      : proof [] ⊤ ∀' ∃' ∃' (<2> ≃ (prod <1> <0>))
+  #reduce 𝟘⁅⊤ ⋀ ⊥⁆
+  #reduce 𝟙⁅⊤ ⋀ ⊥⁆
 
-| prod_distinct_rep    :
-    proof [] ⊤
-      ∀' ∀' ∀' ∀' (prod <3> <1> ≃ prod <2> <0>) ⟹ (<3> ≃ <2> ⋀ <1> ≃ <0>)
+end substitution
 
-example : proof [] ⊤ ⊤ := proof.axm WF.top
+section proofs
 
-lemma proof_WF {Γ : context} {P Q: term} : WF Γ P Ω → proof Γ P Q → WF Γ Q Ω := sorry
--- begin
--- intros wfP prf,
--- induction prf,
--- case proof.axm {exact wfP},
--- case proof.vac {exact WF.top},
--- case proof.abs {exact prf_a},
--- case proof.cut {sorry},
--- end
+  inductive proof : context → term → term → Prop
+  | axm        {Γ φ}         : WF Γ Ω φ → proof Γ φ φ
+  | vac        {Γ φ}         : WF Γ Ω φ → proof Γ φ ⊤
+  | abs        {Γ φ}         : WF Γ Ω φ → proof Γ ⊥ φ
+  | and_intro  {Γ p q r}     : proof Γ p q → proof Γ p r → proof Γ p (q ⋀ r)  
+  | and_left   {Γ} (p q r)   : proof Γ p (q ⋀ r) → proof Γ p q
+  | and_right  {Γ} (p q r)   : proof Γ p (q ⋀ r) → proof Γ p r
+  | or_intro   {Γ p q r}     : proof Γ p r → proof Γ q r → proof Γ (p ⋁ q) r  
+  | or_left    {Γ} (p q r)   : proof Γ (p ⋁ q) r → proof Γ p r
+  | or_right   {Γ} (p q r)   : proof Γ (p ⋁ q) r → proof Γ q r
+  | imp_to_and {Γ p q r}     : proof Γ p (q ⟹ r) → proof Γ (p ⋀ q) r
+  | and_to_imp {Γ p q r}     : proof Γ (p ⋀ q) r → proof Γ p (q ⟹ r)
+  | weakening  {Γ φ ψ B}     : proof Γ φ ψ → proof (list.concat Γ B) φ ψ
+  | cut        {Γ} (φ c ψ)   : proof Γ φ c → proof Γ c ψ → proof Γ φ ψ
+  | all_elim   {Γ p φ B}     : proof Γ p (∀' φ) → proof (B::Γ) p φ
+  | all_intro  {Γ p φ} (B)   : proof (B::Γ) p φ → proof Γ p (∀' φ)
+  | ex_elim    {Γ p φ B}     : proof Γ p (∃' φ) → proof (B::Γ) p φ
+  | ex_intro   {Γ p φ B}     : proof (B::Γ) p φ → proof Γ p (∃' φ)
+  | ext                      : proof [] ⊤ $ ∀' ∀' (∀' (𝟘 ∈ 𝟚) ⇔ (𝟘 ∈ 𝟙)) ⟹ (𝟙 ≃ 𝟘)
+  | prop_ext                 : proof [] ⊤ ∀' ∀' (𝟙 ⇔ 𝟘) ⟹ (𝟚 ≃ 𝟙)
+  | star_unique              : proof [] ⊤ ∀' (𝟙 ≃ ⁎)
+  | pair_exists_rep          : proof [] ⊤ ∀' ∃' ∃' 𝟚 ≃ ⟪𝟙,𝟘⟫
+  | pair_distinct_rep        : proof [] ⊤ ∀' ∀' ∀' ∀' (⟪𝟜,𝟚⟫ ≃ ⟪𝟛,𝟙⟫) ⟹ (𝟜 ≃ 𝟛 ⋀ 𝟚 ≃ 𝟙)
+  | apply      {Γ B} (φ ψ b) : WF Γ B b → proof (B::Γ) φ ψ → proof Γ (φ⁅b⁆) (ψ⁅b⁆)
+  | comp       {Γ φ A}       : WF (A::A::Γ) Ω φ → proof Γ ⊤ (∀' (𝟘 ∈ ⟦φ⟧) ⇔ (φ⁅𝟙⁆))
 
-variables p q r : term
+  prefix ⊢ := proof [] ⊤
+  infix ` ⊢ `:50 := proof []
+  notation φ ` ⊢[` Γ:(foldr `,` (h t, list.cons h t) list.nil) `] ` ψ := proof Γ φ ψ
+  notation `⊢[` Γ:(foldr `,` (h t, list.cons h t) list.nil) `] ` ψ := proof Γ ⊤ ψ
 
-example {Γ : context} : proof Γ ⊤ (q ⟹ r) → proof Γ q r := sorry
--- begin
--- intro h₁,
--- apply @proof.cut Γ q (⊤ ⋀ q) r,
--- apply proof.and_intro,
--- apply proof.vac,
--- apply WF_imp_left,
--- end
+  variables p q : term
 
--- example {Γ : context} : proof Γ ⊤ (p ⋀ q) → proof Γ ⊤ (q ⋀ p) :=
--- λ h₁, proof.and_intro (proof.and_right h₁) (proof.and_left h₁)
-example {Γ : context} : proof Γ ⊤ (p ⋀ q) → proof Γ ⊤ (q ⋀ p) :=
-begin
-intro h₁,
-apply proof.and_intro,
-exact proof.and_right h₁,
-exact proof.and_left h₁,
-end
+  #reduce   ⊢ (p ⋁ ∼p)  -- proof [] ⊤ (or p (imp p ⊥))
+  #reduce q ⊢ (p ⋁ ∼p)  -- proof [] q (or p (imp p ⊥))
+  #reduce   ⊢[Ω,Unit] p -- proof [Ω,Unit] ⊤ p
+  #reduce q ⊢[Ω,Unit] p -- proof [Ω,Unit] q p
 
-def FV {Γ : context} {A : type} (a : term): WF Γ a A → finset ℕ := sorry
--- | _ star       := ∅
--- | _ top        := ∅
--- | _ bot        := ∅
--- | _ (p ⋀ q)    := (FV k p) ∪ (FV k q)
--- | _ (p ⋁ q)    := (FV k p) ∪ (FV k q)
--- | _ (p ⟹ q)    := (FV k p) ⟹ (FV k q)
--- | _ (var m)    := if m≥k then var (m+d) else var m
--- | _ ⟦φ⟧         :=    ⟦FV (k+1) φ⟧
--- | _ (∀' φ)     := ∀' FV (k+1) φ
--- | _ (∃' φ)     := ∃' FV (k+1) φ
--- | _ (a ∈ α)    := (FV k a) ∈ (FV k α)
--- | _ (prod a b) := prod (FV k a) (FV k b)
+  variable {Γ : context}
+  variables φ ψ : term
 
+  lemma WF.proof_left  : proof Γ φ ψ → WF Γ Ω φ := sorry
+  lemma WF.proof_right : proof Γ φ ψ → WF Γ Ω ψ := sorry
+
+end proofs
 
 end TT
